Prove some things about execution

src/Spec/Exec.v
@@ -1,12 +1,15 @@
 Require Import Spec.Proc.
 Require Import Spec.ThreadsState.
 
-Require Import Helpers.KleeneStar.
+Require Import Helpers.TransitionSystem.
+Require Import Helpers.ProofAutomation.
+Require Import Helpers.RecordSet.
 
+Require Import Morphisms.
 Require Import List.
 
-Notation "ts [[  tid := p  ]]" := (thread_upd ts tid (Some p)) (at level 11).
-Notation "ts [[  - tid  ]]" := (thread_upd ts tid None) (at level 11).
+Notation "ts [[ tid  :=  p ]]" := (thread_upd ts tid (Some p)) (at level 11).
+Notation "ts [[ - tid ]]" := (thread_upd ts tid None) (at level 11).
 
 Definition TID := nat.
 Implicit Types (tid:TID).
@@ -17,22 +20,34 @@ Inductive event :=
 Definition trace := list (TID * event).
 Definition add_id tid (evs: list event) : trace := map (pair tid) evs.
 
+Definition etrace {A B} (x: A * B * trace) : trace := let '(_, _, tr) := x in tr.
+
+Instance Set_etrace A B : Setter (etrace (A:=A) (B:=B)).
+Proof.
+  refine {| set := fun f '(a, b, tr) => (a, b, f tr); |};
+    intros;
+    destruct matches.
+Defined.
+
 Section Execution.
   Variable Op:Type.
   Variable State:Type.
-  Variable step: Op -> State -> State -> list event -> Prop.
+  Definition InstStep := Op -> State -> State -> list event -> Prop.
+  Variable step: InstStep.
   Implicit Types (op:Op) (p: proc Op) (s:State) (tr:trace).
 
   Inductive proc_step tid : Relation (proc Op * State * trace) :=
   | exec_op : forall op s s' evs,
       step op s s' evs ->
-      forall p' tr, proc_step tid (Exec (Call op) p', s, tr) (p', s', tr ++ add_id tid evs)
+      forall p' tr, proc_step tid
+                         (Exec (Call op) p', s, tr)
+                         (p', s', tr ++ add_id tid evs)
   .
 
   Notation threads := (threads_state (proc Op)).
   Implicit Types (ts:threads).
 
-  Inductive exec_step : threads * State * trace -> threads * State * trace -> Prop :=
+  Inductive exec_step : Relation (threads * State * trace) :=
   | exec_proc : forall ts p p' tid,
       ts tid = Some p ->
       forall s s' tr tr',
@@ -54,5 +69,43 @@ Section Execution.
   .
 
   Definition exec := kleene_star exec_step.
+
+  Theorem proc_step_prepend : forall tid tr0,
+      Proper (proc_step tid ==> proc_step tid) (set etrace (app tr0)).
+  Proof.
+    unfold Proper, "==>"; intros.
+    cbv [set Set_etrace]; destruct matches; subst.
+    invert H.
+    rewrite app_assoc; eauto using proc_step.
+  Qed.
+
+  Theorem kleene_star_proper : forall A (R: Relation A) (f: A -> A),
+      Proper (R ==> R) f ->
+      Proper (kleene_star R ==> kleene_star R) f.
+  Proof.
+    unfold Proper, "==>"; intros.
+    induction H0; eauto using kleene_star.
+  Qed.
+
+  Theorem proc_step_star_prepend : forall tid tr0,
+      Proper (kleene_star (proc_step tid) ==> kleene_star (proc_step tid))
+             (set etrace (app tr0)).
+  Proof.
+    intros.
+    apply kleene_star_proper.
+    apply proc_step_prepend.
+  Qed.
+
+  Theorem exec_tr_prepend : forall tr0,
+      Proper (exec_step ==> exec_step) (set etrace (app tr0)).
+  Proof.
+    unfold Proper, "==>"; intros.
+    cbv [set Set_etrace]; destruct matches; subst.
+    invert H; eauto using exec_step.
+    eapply exec_proc; eauto.
+    apply (proc_step_prepend tr0) in H7; simpl in *; eauto.
+    apply (proc_step_star_prepend tr0) in H7; simpl in *; eauto.
+    eapply exec_atomic; eauto.
+  Qed.
 
 End Execution.
