src/Helpers/TransitionSystem.v
@@ -1,0 +1,56 @@
+Require Import Instances.
+
+Set Implicit Arguments.
+
+Generalizable Variable R.
+
+Section TransitionSystem.
+  Variable A:Type.
+
+  Definition Relation := A -> A -> Prop.
+  Implicit Types (R:Relation).
+
+  Inductive kleene_star R : Relation :=
+  | star_refl : forall x,
+      kleene_star R x x
+  | star_one : forall x1 x2 x3,
+      R x1 x2 ->
+      kleene_star R x2 x3 ->
+      kleene_star R x1 x3.
+
+  Global Instance kleene_star_PreOrder : PreOrder (kleene_star R).
+  Proof.
+    RelInstance_t.
+    - constructor.
+    - induction H; eauto using kleene_star.
+  Qed.
+
+  Theorem kleene_star_one : forall R x1 x2, R x1 x2 -> kleene_star R x1 x2.
+  Proof.
+    eauto using kleene_star.
+  Qed.
+
+  Global Instance kleene_star_sub : subrelation R (kleene_star R) :=
+    kleene_star_one.
+
+  Definition invariant (I: A -> Prop) R :=
+    forall x1, I x1 ->
+          forall x2, R x1 x2 -> I x2.
+
+  Theorem invariant_star : forall I R,
+      invariant I R ->
+      invariant I (kleene_star R).
+  Proof.
+    unfold invariant; intros.
+    induction H1; eauto.
+  Qed.
+
+  Theorem invariant_star' : forall I R,
+      invariant I (kleene_star R) ->
+      invariant I R.
+  Proof.
+    unfold invariant; intros.
+    eapply H; eauto using kleene_star_one.
+  Qed.
+
+End TransitionSystem.
