src/Spec/TraceIncl.v
@@ -1,0 +1,19 @@
+Require Import Spec.Proc.
+Require Import Spec.Exec.
+
+Section Semantics.
+  Variable Op:Type.
+  Variable State:Type.
+  Variable step: InstStep Op State.
+
+  Notation exec := (exec step).
+
+  Implicit Types (op:Op) (p: proc Op) (s:State) (tr:trace).
+
+  Definition trace_incl p1 p2 :=
+    forall ts tid,
+    forall s s' tr tr' ts1',
+      exec (ts [[tid := p1]], s, tr) (ts1', s', tr') ->
+      exists ts2', exec (ts [[tid := p2]], s, tr) (ts2', s', tr').
+
+End Semantics.
